one inversion working

theories/Logic/cpl_trees.v
@@ -11,10 +11,13 @@ Require Import List.
 Import ListNotations.
 Require Import Coq.Logic.ProofIrrelevance.
 Require Import Coq.Logic.Eqdep_dec.
+Require Import Arith.
 
 
 Inductive cpl_tree : Type :=
 | leaf : forall (OC : constraint) (gamma delta : list formula) (alpha : ordinal), cpl_tree
+
+| deg_up : forall {OC : constraint} {gamma delta : list formula} (alpha beta : ordinal) (T' : cpl_tree), cpl_tree 
 
 | con_l : forall {OC : constraint} {gamma delta : list formula} (phi : formula) {alpha : ordinal} (T' : cpl_tree), cpl_tree
 
@@ -49,6 +52,7 @@ Definition cpl_tree_left (T : cpl_tree) : list formula :=
 match T with
 | leaf OC gamma delta alpha => gamma
 
+| @deg_up OC gamma delta alpha beta T' => gamma 
 
 | @con_l OC gamma delta phi alpha T' => phi :: gamma
 
@@ -84,6 +88,8 @@ Definition cpl_tree_right (T : cpl_tree) : list formula :=
 match T with
 | leaf OC gamma delta alpha => delta
 
+| @deg_up OC gamma delta alpha beta T' => delta
+
 | @con_l OC gamma delta phi alpha T' => delta
 
 | @con_r OC gamma delta phi alpha T' => phi :: delta
@@ -117,6 +123,8 @@ end.
 Definition cpl_tree_constraint (T : cpl_tree) : constraint :=
 match T with
 | leaf OC gamma delta alpha => OC
+
+| @deg_up OC gamma delta alpha beta T' => OC
 
 | @con_l OC gamma delta phi alpha T' => OC
 
@@ -152,6 +160,8 @@ Definition cpl_tree_deg (T : cpl_tree) : ordinal :=
 match T with
 | leaf OC gamma delta alpha => alpha
 
+| @deg_up OC gamma delta alpha beta T' => omax alpha beta
+
 | @con_l OC gamma delta phi alpha T' => alpha
 
 | @con_r OC gamma delta phi alpha T' => alpha
@@ -185,6 +195,8 @@ Fixpoint cpl_leaves (T : cpl_tree) : (list (constraint * list formula * list for
 match T with
 | leaf OC gamma delta alpha => [(OC, gamma, delta, alpha)]
 
+| @deg_up OC gamma delta alpha beta T' => (cpl_leaves T')
+
 | @con_l OC gamma delta phi alpha T' => (cpl_leaves T')
 
 | @con_r OC gamma delta phi alpha T' => (cpl_leaves T')
@@ -215,23 +227,61 @@ match T with
 | @cut OC gamma delta phi alpha1 alpha2 T1 T2 => (cpl_leaves T1) ++ (cpl_leaves T2)
 end.
 
+
+Fixpoint cpl_tree_depth (T : cpl_tree) : nat :=
+match T with
+| leaf OC gamma delta alpha => 0
+
+| @deg_up OC gamma delta alpha beta T' => cpl_tree_depth T'
+
+| @con_l OC gamma delta phi alpha T' => cpl_tree_depth T'
+
+| @con_r OC gamma delta phi alpha T' => cpl_tree_depth T'
+
+
+| @ex_l OC gamma delta n alpha T' => cpl_tree_depth T'
+
+| @ex_r OC gamma delta n alpha T' => cpl_tree_depth T'
+
+
+| @wkn_l OC gamma delta phi alpha T' => S (cpl_tree_depth T')
+
+| @wkn_r OC gamma delta phi alpha T' => S (cpl_tree_depth T')
+
+| @rst OC gamma delta kappa alpha T' => S (cpl_tree_depth T')
+
+
+| @bnd_l OC gamma delta phi lambda kappa alpha T' => S (cpl_tree_depth T')
+
+| @bnd_r OC gamma delta phi lambda kappa alpha T' => S (cpl_tree_depth T')
+
+
+| @imp_l OC gamma delta phi psi alpha1 alpha2 T1 T2 => S (max (cpl_tree_depth T1) (cpl_tree_depth T2))
+
+| @imp_r OC gamma delta phi psi alpha T' => S (cpl_tree_depth T')
+
+
+| @cut OC gamma delta phi alpha1 alpha2 T1 T2 => S (max (cpl_tree_depth T1) (cpl_tree_depth T2))
+end.
+
 Lemma cpl_tree_eq_dec : forall (T1 T2 : cpl_tree), {T1 = T2} + {T1 <> T2}.
 Proof.
 induction T1;
 destruct T2.
 
-2-14 : right; discriminate.
-3-15 : right; discriminate.
-4-16 : right; discriminate.
-5-17 : right; discriminate.
-6-18 : right; discriminate.
-7-19 : right; discriminate.
-8-20 : right; discriminate.
-9-21 : right; discriminate.
-10-22 : right; discriminate.
-11-23 : right; discriminate.
-12-24 : right; discriminate.
-13-25 : right; discriminate.
+2-15 : right; discriminate.
+3-16 : right; discriminate.
+4-17 : right; discriminate.
+5-18 : right; discriminate.
+6-19 : right; discriminate.
+7-20 : right; discriminate.
+8-21 : right; discriminate.
+9-22 : right; discriminate.
+10-23 : right; discriminate.
+11-24 : right; discriminate.
+12-25 : right; discriminate.
+13-26 : right; discriminate.
+14-27 : right; discriminate.
 
 all : try destruct (nat_eq_dec n n0) as [EQN | NE];
       try destruct (IHT1 T2) as [EQ | NE];
@@ -250,6 +300,7 @@ all : try destruct (nat_eq_dec n n0) as [EQN | NE];
       try destruct (form_eq_dec phi phi0) as [EQT1 | NE];
 			try destruct (form_eq_dec psi psi0) as [EQT2 | NE];
 			try destruct (ordinal_eq_dec alpha alpha0) as [EQA | NE];
+      try destruct (ordinal_eq_dec beta beta0) as [EQB | NE];
       try destruct (ordinal_eq_dec alpha1 alpha0) as [EQA1 | NE];
       try destruct (ordinal_eq_dec alpha2 alpha3) as [EQA2 | NE];
 			try destruct (nat_eq_dec kappa kappa0) as [EQK | NE];
@@ -266,10 +317,11 @@ Qed.
 
 Definition semi_applicable (OC : constraint) (T : cpl_tree) : Prop := (incl (flat_map vars_in (cpl_tree_left T)) (OC_list OC)) * (incl (flat_map vars_in (cpl_tree_right T)) (OC_list OC)).
 
-
 Fixpoint structured (T : cpl_tree) : Type :=
 match T with
 | leaf OC gamma delta alpha => semi_applicable OC T
+
+| @deg_up OC gamma delta alpha beta T' => structured T' * (semi_applicable OC T * (cpl_tree_left T' = gamma) * (cpl_tree_right T' = delta) * (cpl_tree_constraint T' = OC) * (cpl_tree_deg T' = alpha))
 
 | @con_l OC gamma delta phi alpha T' => structured T' * (semi_applicable OC T * (cpl_tree_left T' = phi :: phi :: gamma) * (cpl_tree_right T' = delta) * (cpl_tree_constraint T' = OC) * (cpl_tree_deg T' = alpha))
 
@@ -300,7 +352,7 @@ match T with
 | @cut OC gamma delta phi alpha1 alpha2 T1 T2 => (structured T1 * structured T2) * (semi_applicable OC T * (cpl_tree_left T1 = gamma) * (cpl_tree_right T1 = phi :: delta) * (cpl_tree_constraint T1 = OC) * (cpl_tree_left T2 = phi :: gamma) * (cpl_tree_right T2 = delta) * (cpl_tree_constraint T2 = OC) * (cpl_tree_deg T1 = alpha1) * (cpl_tree_deg T2 = alpha2))
 end.
 
-Lemma test :
+Lemma cpl_last_is_showable :
     forall (T : cpl_tree),
         structured T ->
             (forall L,
@@ -312,19 +364,23 @@ induction T;
 intros Tstr LEAF.
 
 1 : destruct Tstr as [TG_app TD_app].
-2-7 : destruct Tstr as [Tstr [[[[[TG_app TD_app] TG] TD] TOC] TDeg]].
-8 : destruct Tstr as [Tstr [[[[[[[TG_app TD_app] TG] TD] KNING] KNIND] [KIN TOC]] TDeg]].
-9 : destruct Tstr as [Tstr [[[[[[TG_app TD_app] TG] TD] TOC] TOC_rel] TDeg]].
-10 : destruct Tstr as [Tstr [[[[[[TG_app TD_app] TG] TD] [NEW [KIN TOC]]] [NING NIND]] TDeg]].
-11 : destruct Tstr as [[T1str T2str] [[[[[[[[[TG_app TD_app] T1G] T1D] T1OC] T2G] T2D] T2OC] T1Deg] T2Deg]].
-12 : destruct Tstr as [Tstr [[[[[TG_app TD_app] TG] TD] TOC] TDeg]].
-13 : destruct Tstr as [[T1str T2str] [[[[[[[[[TG_app TD_app] T1G] T1D] T1OC] T2G] T2D] T2OC] T1Deg] T2Deg]].
+2-8 : destruct Tstr as [Tstr [[[[[TG_app TD_app] TG] TD] TOC] TDeg]].
+9 : destruct Tstr as [Tstr [[[[[[[TG_app TD_app] TG] TD] KNING] KNIND] [KIN TOC]] TDeg]].
+10 : destruct Tstr as [Tstr [[[[[[TG_app TD_app] TG] TD] TOC] TOC_rel] TDeg]].
+11 : destruct Tstr as [Tstr [[[[[[TG_app TD_app] TG] TD] [NEW [KIN TOC]]] [NING NIND]] TDeg]].
+12 : destruct Tstr as [[T1str T2str] [[[[[[[[[TG_app TD_app] T1G] T1D] T1OC] T2G] T2D] T2OC] T1Deg] T2Deg]].
+13 : destruct Tstr as [Tstr [[[[[TG_app TD_app] TG] TD] TOC] TDeg]].
+14 : destruct Tstr as [[T1str T2str] [[[[[[[[[TG_app TD_app] T1G] T1D] T1OC] T2G] T2D] T2OC] T1Deg] T2Deg]].
 
 all : unfold provable in *;
       unfold cpl_tree_constraint, cpl_tree_left, cpl_tree_right, cpl_tree_deg.
 
 1 : specialize (LEAF (OC, gamma, delta, alpha) (or_introl eq_refl)).
     apply LEAF.
+
+1 : apply ptree_deg_up.
+    rewrite <- TG, <- TD, <- TOC, <- TDeg.
+    apply (IHT Tstr LEAF).
 
 1 : apply ptree_con_l.
     rewrite <- TG, <- TD, <- TOC, <- TDeg.
@@ -382,16 +438,762 @@ all : unfold provable in *;
     apply (IHT2 T2str (fun L IN => LEAF L (in_or_app _ _ _ (or_intror IN)))).
 Qed.
 
+Definition T_shows (T : cpl_tree) (OC : constraint) (gamma delta : list formula) (alpha : ordinal) (d : nat) : Type :=
+  (structured T) * (cpl_tree_left T = gamma) * (cpl_tree_right T = delta) * (cpl_tree_constraint T = OC) * (cpl_tree_deg T = alpha) * (cpl_tree_depth T = d).
+
+Definition showable (OC : constraint) (gamma delta : list formula) (alpha : ordinal) (d : nat) : Type :=
+  {T : cpl_tree & (T_shows T OC gamma delta alpha d)}.
+
+Lemma structured_OC_semiapp :
+  forall (T : cpl_tree),
+      structured T ->
+          semi_applicable (cpl_tree_constraint T) T.
+Proof.
+induction T;
+intros Tstr.
+
+1 : destruct Tstr as [TG_app TD_app].
+2-8 : destruct Tstr as [Tstr [[[[[TG_app TD_app] TG] TD] TOC] TDeg]].
+9 : destruct Tstr as [Tstr [[[[[[[TG_app TD_app] TG] TD] KNING] KNIND] [KIN TOC]] TDeg]].
+10 : destruct Tstr as [Tstr [[[[[[TG_app TD_app] TG] TD] TOC] TOC_rel] TDeg]].
+11 : destruct Tstr as [Tstr [[[[[[TG_app TD_app] TG] TD] [NEW [KIN TOC]]] [NING NIND]] TDeg]].
+12 : destruct Tstr as [[T1str T2str] [[[[[[[[[TG_app TD_app] T1G] T1D] T1OC] T2G] T2D] T2OC] T1Deg] T2Deg]].
+13 : destruct Tstr as [Tstr [[[[[TG_app TD_app] TG] TD] TOC] TDeg]].
+14 : destruct Tstr as [[T1str T2str] [[[[[[[[[TG_app TD_app] T1G] T1D] T1OC] T2G] T2D] T2OC] T1Deg] T2Deg]].
+
+all : repeat split;
+      unfold cpl_tree_left, cpl_tree_right, flat_map, vars_in;
+      fold vars_in (flat_map vars_in);
+      try apply TG_app;
+      try apply TD_app.
+Qed.
+
+
+Lemma cpl_tree_deg_up :
+  forall {OC : constraint} {gamma delta : list formula} {alpha beta : ordinal} {d : nat},
+      showable OC gamma delta alpha d ->
+          showable OC gamma delta (omax alpha beta) d.
+Proof.
+intros OC gamma delta alpha beta d [T [[[[[Tstr Tgam] Tdelt] Tcon] Tdeg] Tdep]].
+subst.
+refine (existT _ (deg_up (cpl_tree_deg T) beta T) _).
+repeat split;
+try assumption.
+1 : apply (fst (structured_OC_semiapp _ Tstr)).
+1 : apply (snd (structured_OC_semiapp _ Tstr)).
+Qed.
+
+Lemma cpl_tree_con_l :
+  forall {OC : constraint} {gamma delta : list formula} {phi : formula} {alpha : ordinal} {d : nat},
+      showable OC (phi :: phi :: gamma) delta alpha d ->
+          showable OC (phi :: gamma) delta alpha d.
+Proof.
+intros OC gamma delta phi alpha d [T [[[[[Tstr Tgam] Tdelt] Tcon] Tdeg] Tdep]].
+subst.
+refine (existT _ (con_l phi T) _).
+repeat split;
+try assumption.
+1 : refine (incl_tran (@flat_map_incl _ _ form_eq_dec nat_eq_dec vars_in _ (phi :: phi :: gamma) (fun (A : formula) (IN : In A (phi :: gamma)) => (or_intror IN))) _).
+  rewrite <- Tgam.
+  apply (fst (structured_OC_semiapp _ Tstr)).
+1 : apply (snd (structured_OC_semiapp _ Tstr)).
+Qed.
+
+Lemma cpl_tree_con_r :
+  forall {OC : constraint} {gamma delta : list formula} {phi : formula} {alpha : ordinal} {d : nat},
+      showable OC gamma (phi :: phi :: delta) alpha d ->
+          showable OC gamma (phi :: delta) alpha d.
+Proof.
+intros OC gamma delta phi alpha d [T [[[[[Tstr Tgam] Tdelt] Tcon] Tdeg] Tdep]].
+subst.
+refine (existT _ (con_r phi T) _).
+repeat split;
+try assumption.
+1 : apply (fst (structured_OC_semiapp _ Tstr)).
+1 : refine (incl_tran (@flat_map_incl _ _ form_eq_dec nat_eq_dec vars_in _ (phi :: phi :: delta) (fun (A : formula) (IN : In A (phi :: delta)) => (or_intror IN))) _).
+    rewrite <- Tdelt.
+    apply (snd (structured_OC_semiapp _ Tstr)).
+Qed.
+
+Lemma cpl_tree_ex_l : 
+  forall {OC : constraint} {gamma delta : list formula} {n : nat} {alpha : ordinal} {d : nat},
+      showable OC gamma delta alpha d ->
+          showable OC (bury gamma n) delta alpha d.
+Proof.
+intros OC gamma delta n alpha d [T [[[[[Tstr Tgam] Tdelt] Tcon] Tdeg] Tdep]].
+subst.
+refine (existT _ (ex_l n T) _).
+repeat split;
+try assumption.
+1 : refine (incl_tran (fun A => proj1 (flat_map_bury_incl A)) (fst (structured_OC_semiapp _ Tstr))).
+1 : apply (snd (structured_OC_semiapp _ Tstr)).
+Qed.
+
+Lemma cpl_tree_ex_r : 
+  forall {OC : constraint} {gamma delta : list formula} {n : nat} {alpha : ordinal} {d : nat},
+      showable OC gamma delta alpha d ->
+          showable OC gamma (bury delta n) alpha d.
+Proof.
+intros OC gamma delta n alpha d [T [[[[[Tstr Tgam] Tdelt] Tcon] Tdeg] Tdep]].
+subst.
+refine (existT _ (ex_r n T) _).
+repeat split;
+try assumption.
+1 : apply (fst (structured_OC_semiapp _ Tstr)).
+1 : refine (incl_tran (fun A => proj1 (flat_map_bury_incl A)) (snd (structured_OC_semiapp _ Tstr))).
+Qed.
+
+Lemma cpl_tree_wkn_l : 
+  forall {OC : constraint} {gamma delta : list formula} {phi : formula} {alpha: ordinal} {d : nat},
+      incl (vars_in phi) (OC_list OC) ->
+          showable OC gamma delta alpha d ->
+              showable OC (phi :: gamma) delta alpha (S d).
+Proof.
+intros OC gamma delta phi alpha d SUB [T [[[[[Tstr Tgam] Tdelt] Tcon] Tdeg] Tdep]].
+subst.
+refine (existT _ (wkn_l phi T) _).
+repeat split;
+try assumption.
+1 : apply (incl_app SUB (fst (structured_OC_semiapp _ Tstr))).
+1 : apply (snd (structured_OC_semiapp _ Tstr)).
+Qed.
+
+Lemma cpl_tree_wkn_r : 
+  forall {OC : constraint} {gamma delta : list formula} {phi : formula} {alpha: ordinal} {d : nat},
+      incl (vars_in phi) (OC_list OC) ->
+          showable OC gamma delta alpha d ->
+              showable OC gamma (phi :: delta) alpha (S d).
+Proof.
+intros OC gamma delta phi alpha d SUB [T [[[[[Tstr Tgam] Tdelt] Tcon] Tdeg] Tdep]].
+subst.
+refine (existT _ (wkn_r phi T) _).
+repeat split;
+try assumption.
+1 : apply (fst (structured_OC_semiapp _ Tstr)).
+1 : apply (incl_app SUB (snd (structured_OC_semiapp _ Tstr))).
+Qed.
+
+Lemma cpl_tree_weaken_left : 
+  forall {gamma delta sigma : list formula} {OC : constraint} {alpha: ordinal} {d : nat},
+      incl (flat_map vars_in sigma) (OC_list OC) ->
+          showable OC gamma delta alpha d ->
+              showable OC (gamma ++ sigma) delta alpha (length sigma + d).
+Proof.
+intros gamma delta sigma.
+revert gamma delta.
+apply (rev_ind_type (fun sigma => forall (gamma delta : list formula) (OC : constraint) (alpha : ordinal) (d : nat), incl (flat_map vars_in sigma) (OC_list OC) -> showable OC gamma delta alpha d -> showable OC (gamma ++ sigma) delta alpha (length sigma + d))).
+- intros gamma delta OC alpha d SUB Tshow.
+  rewrite app_nil_r.
+  apply Tshow.
+- intros phi sigma' IND gamma delta OC alpha d SUB Tshow.
+  rewrite app_assoc.
+  rewrite <- (app_nil_l ((gamma ++ sigma') ++ [phi])), <- (@bury_type _ phi [] (gamma ++ sigma')), app_nil_l, app_length.
+  unfold length at 3.
+  rewrite <- plus_n_Sm, <- plus_n_O, plus_Sn_m.
+  apply cpl_tree_ex_l, cpl_tree_wkn_l, IND, Tshow;
+  rewrite flat_map_app in SUB.
+  refine (fun o IN => SUB _ (in_or_app _ (flat_map vars_in [phi]) _ (or_intror (in_or_app _ _ _ (or_introl IN))))).
+  refine (fun o IN => SUB _ (in_or_app _ (flat_map vars_in [phi]) _ (or_introl IN))).
+Qed.
+
+Lemma cpl_tree_weaken_right : 
+  forall {gamma delta pi : list formula} {OC : constraint} {alpha: ordinal} {d : nat},
+      incl (flat_map vars_in pi) (OC_list OC) ->
+          showable OC gamma delta alpha d ->
+              showable OC gamma (delta ++ pi) alpha (length pi + d).
+Proof.
+intros gamma delta pi.
+revert gamma delta.
+apply (rev_ind_type (fun pi => forall (gamma delta : list formula) (OC : constraint) (alpha : ordinal) (d : nat), incl (flat_map vars_in pi) (OC_list OC) -> showable OC gamma delta alpha d -> showable OC gamma (delta ++ pi) alpha (length pi + d))).
+- intros gamma delta OC alpha d SUB Tshow.
+  rewrite app_nil_r.
+  apply Tshow.
+- intros phi pi' IND gamma delta OC alpha d SUB Tshow.
+  rewrite app_assoc.
+  rewrite <- (app_nil_l ((delta ++ pi') ++ [phi])), <- (@bury_type _ phi [] (delta ++ pi')), app_nil_l, app_length.
+  unfold length at 3.
+  rewrite <- plus_n_Sm, <- plus_n_O, plus_Sn_m.
+  apply cpl_tree_ex_r, cpl_tree_wkn_r, IND, Tshow;
+  rewrite flat_map_app in SUB.
+  refine (fun o IN => SUB _ (in_or_app _ (flat_map vars_in [phi]) _ (or_intror (in_or_app _ _ _ (or_introl IN))))).
+  refine (fun o IN => SUB _ (in_or_app _ (flat_map vars_in [phi]) _ (or_introl IN))).
+Qed.
+
+Lemma cpl_tree_reset : 
+  forall {gamma delta : list formula} {OC : constraint} {kappa : ovar} {alpha: ordinal} {d : nat},
+      ~ In kappa (flat_map vars_used gamma) ->
+          ~ In kappa (flat_map vars_used delta) ->
+              OC_elt OC kappa ->
+                  showable (restriction OC (children OC kappa) (children_subset OC kappa)) gamma delta alpha d ->
+                      showable OC gamma delta alpha (S d).
+Proof.
+intros gamma delta OC kappa alpha d NING NIND ELT [T [[[[[Tstr Tgam] Tdelt] Tcon] Tdeg] Tdep]].
+subst.
+refine (existT _ (rst kappa T) _).
+repeat split;
+try assumption.
+1 : apply (incl_tran (fst (structured_OC_semiapp _ Tstr))).
+2 : apply (incl_tran (snd (structured_OC_semiapp _ Tstr))).
+1,2 : rewrite Tcon;
+      apply incl_filter.
+Qed.
+
+Lemma cpl_tree_bnd_l : 
+  forall {OC : constraint} {gamma delta : list formula} {phi : formula} {lambda kappa : ovar} {alpha : ordinal} {d : nat},
+      OC_rel OC lambda kappa = true ->
+          showable OC (phi :: gamma) delta alpha d ->
+              showable OC ((bnd lambda kappa phi) :: gamma) delta alpha (S d).
+Proof.
+intros OC gamma delta phi lambda kappa alpha d rel [T [[[[[Tstr Tgam] Tdelt] Tcon] Tdeg] Tdep]].
+subst.
+refine (existT _ (bnd_l phi lambda kappa T) _).
+repeat split;
+try assumption.
+1 : { intros o IN.
+    apply in_app_or in IN as [[IN1 | IN2] | IN3].
+    - subst.
+      apply (OC_null _ _ _ rel).
+    - apply in_remove in IN2 as [IN2 _].
+      apply (fst (structured_OC_semiapp _ Tstr)).
+      rewrite Tgam.
+      apply in_or_app, or_introl, IN2.
+    - apply (fst (structured_OC_semiapp _ Tstr)).
+      rewrite Tgam.
+      apply in_or_app, or_intror, IN3. }
+1 : apply (snd (structured_OC_semiapp _ Tstr)).
+Qed.
+
+Lemma cpl_tree_bnd_r : 
+  forall {OC : constraint} {gamma delta : list formula} {phi : formula} {lambda kappa : ovar} {alpha : ordinal} {d : nat} (NEW : ~ OC_elt OC lambda) (KIN : OC_elt OC kappa),
+      ~ In lambda (flat_map vars_used gamma) ->
+          ~ In lambda (flat_map vars_used (phi :: delta)) ->
+              showable (add_fresh_child OC lambda kappa NEW KIN) gamma (phi :: delta) alpha d ->
+                  showable OC gamma ((bnd lambda kappa phi) :: delta) alpha (S d).
+Proof.
+intros OC gamma delta phi lambda kappa alpha d NEW KIN NING NIND [T [[[[[Tstr Tgam] Tdelt] Tcon] Tdeg] Tdep]].
+subst.
+refine (existT _ (bnd_r phi lambda kappa T) _).
+repeat split;
+try assumption.
+3 : refine (existT _ NEW (existT _ KIN Tcon)).
+1 : intros o IN.
+  pose proof ((fst (structured_OC_semiapp _ Tstr)) o IN) as PG_app.
+  rewrite Tcon in PG_app.
+  unfold OC_list, add_fresh_child, projT1 in PG_app.
+  destruct PG_app as [EQ | PG_app].
+  subst.
+  contradiction (NING (vars_in_list_is_used _ _ IN)).
+  apply PG_app.    
+1 : { intros o [EQ | IN].
+    1 : subst.
+        apply KIN.
+    1 : apply in_app_or in IN as [IN1 | IN2].
+        apply  in_remove in IN1 as [IN1 _].
+    all : pose proof ((snd (structured_OC_semiapp _ Tstr)) o) as PD_app;
+          rewrite Tdelt, Tcon in PD_app;
+          try specialize (PD_app (in_or_app _ _ _ (or_introl IN1)));
+          try specialize (PD_app (in_or_app _ _ _ (or_intror IN2)));
+          unfold OC_list, add_fresh_child, projT1 in PD_app;
+          destruct PD_app as [EQ | PD_app];
+          subst.
+    1 : contradiction (NIND (in_or_app _ _ _ (or_introl (vars_in_is_used _ _ IN1)))).
+    1 : apply PD_app.
+    1 : contradiction (NIND (in_or_app _ _ _ (or_intror (vars_in_list_is_used _ _  IN2)))).
+    1 : apply PD_app. }
+Qed.
+
+Lemma cpl_tree_imp_l : 
+  forall {OC : constraint} {gamma delta : list formula} {phi psi : formula} {alpha1 alpha2 : ordinal} {d1 d2 : nat},
+      showable OC (psi :: gamma) delta alpha1 d1 ->
+          showable OC gamma (phi :: delta) alpha2 d2 ->
+              showable OC ((imp phi psi) :: gamma) delta (omax alpha1 alpha2) (S (max d1 d2)).
+Proof.
+intros OC gamma delta phi psi alpha1 alpha2 d1 d2 [T1 [[[[[T1str T1gam] T1delt] T1con] T1deg] T1dep]] [T2 [[[[[T2str T2gam] T2delt] T2con] T2deg] T2dep]].
+subst.
+refine (existT _ (imp_l phi psi T1 T2) _).
+repeat split;
+try assumption.
+1 : intros o IN.
+  repeat apply in_app_or in IN as [IN | IN].
+1 : rewrite <- T2con.
+    apply (snd (structured_OC_semiapp _ T2str)).
+    rewrite T2delt.
+    apply (in_or_app _ _ _ (or_introl IN)).
+1 : apply (fst (structured_OC_semiapp _ T1str)).
+    rewrite T1gam.
+    apply (in_or_app _ _ _ (or_introl IN)).
+1 : rewrite <- T2con.
+    apply (fst (structured_OC_semiapp _ T2str)), IN.
+1 : apply (snd (structured_OC_semiapp _ T1str)).
+Qed.
+
+Lemma cpl_tree_imp_r : 
+  forall {OC : constraint} {gamma delta : list formula} {phi psi : formula} {alpha : ordinal} {d : nat},
+      showable OC (phi :: gamma) (psi :: delta) alpha d ->
+          showable OC gamma ((imp phi psi) :: delta) alpha (S d).
+Proof.
+intros OC gamma delta phi psi alpha d [T [[[[[Tstr Tgam] Tdelt] Tcon] Tdeg] Tdep]].
+subst.
+refine (existT _ (imp_r phi psi T) _).
+repeat split;
+try assumption.
+1 : refine (incl_tran _ (fst (structured_OC_semiapp _ Tstr))).
+  rewrite Tgam.
+  apply (@flat_map_incl _ _ form_eq_dec nat_eq_dec vars_in _ (phi :: gamma) (fun (A : formula) (IN : In A gamma) => (or_intror IN))).
+1 : intros o IN.
+  repeat apply in_app_or in IN as [IN | IN].
+1 : apply (fst (structured_OC_semiapp _ Tstr)).
+    rewrite Tgam.
+    apply (in_or_app _ _ _ (or_introl IN)).
+1 : apply (snd (structured_OC_semiapp _ Tstr)).
+    rewrite Tdelt.
+    apply (in_or_app _ _ _ (or_introl IN)).
+1 : apply (snd (structured_OC_semiapp _ Tstr)).
+    rewrite Tdelt.
+    apply (in_or_app _ _ _ (or_intror IN)).
+Qed.
+
+Lemma cpl_tree_cut : 
+  forall {OC : constraint} {gamma delta : list formula} {phi : formula} {alpha1 alpha2 : ordinal} {d1 d2 : nat},
+      showable OC gamma (phi :: delta) alpha1 d1 ->
+          showable OC (phi :: gamma) delta alpha2 d2 ->
+              showable OC gamma delta (omax (omax alpha1 alpha2) (oadd (num_conn phi) (cast (nat_ord 1)))) (S (max d1 d2)).
+Proof.
+intros OC gamma delta phi alpha1 alpha2 d1 d2 [T1 [[[[[T1str T1gam] T1delt] T1con] T1deg] T1dep]] [T2 [[[[[T2str T2gam] T2delt] T2con] T2deg] T2dep]].
+subst.
+refine (existT _ (cut phi T1 T2) _).
+repeat split;
+try assumption.
+1 : apply (fst (structured_OC_semiapp _ T1str)).
+1 : rewrite <- T2con.
+    apply (snd (structured_OC_semiapp _ T2str)).
+Qed.
+
+Lemma commutative_left_aux :
+  forall {LN : list nat} {gamma1 gamma2 delta : list formula} {OC : constraint} {alpha: ordinal} {d : nat},
+      (set_bury gamma1 LN = gamma2) ->
+          showable OC gamma1 delta alpha d ->
+              showable OC gamma2 delta alpha d.
+Proof.
+induction LN;
+intros gamma1 gamma2 delta OC alpha d EQ Tshow.
+- unfold set_bury in EQ.
+  subst.
+  apply Tshow.
+- unfold set_bury in EQ;
+  fold @set_bury in EQ.
+  apply (IHLN _ _ _ _ _ _ EQ), cpl_tree_ex_l, Tshow.
+Qed.
+
+Lemma cpl_tree_comm_left :
+  forall {gamma1 gamma2 delta : list formula} {OC : constraint} {alpha : ordinal} {d : nat},
+      (perm gamma1 gamma2) ->
+          showable OC gamma1 delta alpha d ->
+              showable OC gamma2 delta alpha d.
+Proof.
+intros gamma1 gamma2 delta OC alpha d perm SHOW.
+pose proof (set_bury_eq_perm perm) as [LN EQ].
+apply (commutative_left_aux EQ SHOW).
+Defined.
+
+Lemma prove_dups_left_aux :
+  forall {n : nat} {gamma delta : list formula} {OC : constraint} {alpha: ordinal} {d : nat},
+      length gamma = n ->
+          showable OC gamma delta alpha d ->
+              showable OC (nodup form_eq_dec gamma) delta alpha d.
+Proof.
+induction n;
+intros gamma delta OC alpha d EQ Tshow.
+- destruct gamma.
+  + apply Tshow.
+  + inversion EQ.
+- case (no_dup_dec_cases form_eq_dec gamma) as [NDG | DG].
+  + rewrite (nodup_fixed_point _ NDG).
+    apply Tshow.
+  + destruct (has_dups_split form_eq_dec DG) as [A [gamma1 [gamma2 [gamma3 EQL]]]].
+    rewrite EQL in *.
+    assert (length (A :: gamma1 ++ gamma2 ++ gamma3) = n) as LEN.
+    { rewrite app_length in EQ.
+      unfold length in *;
+      fold (@length formula) in *.
+      repeat rewrite app_length in *.
+      unfold length in EQ;
+      fold (@length formula) in EQ.
+      repeat rewrite <- plus_n_Sm in EQ.
+      lia. }
+    apply (cpl_tree_comm_left (perm_sym (perm_nodup form_eq_dec double_perm_head))).
+    rewrite nodup_double_cons.
+    apply (IHn _ _ _ _ _ LEN (cpl_tree_con_l (cpl_tree_comm_left (double_perm_head) Tshow))).
+Qed.
+
+Lemma cpl_tree_nodups_left :
+  forall {gamma delta : list formula} {OC : constraint} {alpha: ordinal} {d : nat},
+      showable OC gamma delta alpha d ->
+          showable OC (nodup form_eq_dec gamma) delta alpha d.
+Proof.
+intros gamma delta OC alpha d Tshow.
+apply (prove_dups_left_aux eq_refl Tshow).
+Qed.
+
+Lemma prove_extras_left_aux :
+  forall {n : nat} {gamma delta : list formula} {OC : constraint} {alpha: ordinal} {d : nat},
+      length gamma = n ->
+          showable OC (nodup form_eq_dec gamma) delta alpha d ->
+              {d' : nat & showable OC gamma delta alpha d'}.
+Proof.
+induction n;
+intros gamma delta OC alpha d EQ Tshow.
+- destruct gamma.
+  apply (existT _ d Tshow).
+  inversion EQ.
+- case (no_dup_dec_cases form_eq_dec gamma) as [NDG | DG].
++ rewrite <- (nodup_fixed_point form_eq_dec NDG).
+  apply (existT _ d Tshow).
++ destruct (has_dups_split form_eq_dec DG) as [A [gamma1 [gamma2 [gamma3 EQL]]]].
+  subst.
+  destruct (@nodup_split_perm _ form_eq_dec (A :: A :: gamma1 ++ gamma2 ++ gamma3)) as [sigma [PERM SUB]].
+  assert (incl (flat_map vars_in sigma) (OC_list OC)) as SUB'.
+  { destruct Tshow as [T [[[[[Tstr Tgam] Tdelt] Tcon] Tdeg] Tdep]].
+    refine (incl_tran (@flat_map_incl _ _ form_eq_dec nat_eq_dec _ _ _ (incl_tran SUB (incl_tran (fun B IN => perm_in form_eq_dec (perm_sym double_perm_head) _ IN) (fun B IN => proj2 (nodup_In _ _ _) IN)))) _).
+    rewrite <- Tgam, <- Tcon.
+    apply (fst (structured_OC_semiapp _ Tstr)). }
+  apply (existT _ (length sigma + d) (cpl_tree_comm_left (perm_trans _ _ _ (perm_sym PERM) (perm_sym double_perm_head)) (cpl_tree_weaken_left SUB' ((cpl_tree_comm_left (perm_nodup form_eq_dec double_perm_head)) Tshow)))).
+Qed.
+
+Lemma cpl_tree_redups_left :
+  forall {gamma delta : list formula} {OC : constraint} {alpha: ordinal} {d : nat},
+      showable OC (nodup form_eq_dec gamma) delta alpha d ->
+          {d' : nat & showable OC gamma delta alpha d'}.
+Proof.
+intros gamma delta OC alpha d Tshow.
+apply (prove_extras_left_aux eq_refl Tshow).
+Qed.
+
+Lemma cpl_tree_equiv_left :
+  forall {gamma1 gamma2 delta : list formula} {OC : constraint} {alpha : ordinal} {d : nat},
+      (forall A : formula, In A gamma1 <-> In A gamma2) ->
+          showable OC gamma1 delta alpha d ->
+              {d' : nat & showable OC gamma2 delta alpha d'}.
+Proof.
+intros gamma1 gamma2 delta OC alpha d EQUIV Tshow.
+apply (cpl_tree_redups_left ((cpl_tree_comm_left (equiv_nodup_perm form_eq_dec EQUIV)) (cpl_tree_nodups_left Tshow))).
+Qed.
+
+Lemma commutative_right_aux :
+  forall {LN : list nat} {gamma delta1 delta2 : list formula} {OC : constraint} {alpha: ordinal} {d : nat},
+      (set_bury delta1 LN = delta2) ->
+          showable OC gamma delta1 alpha d ->
+              showable OC gamma delta2 alpha d.
+Proof.
+induction LN;
+intros gamma1 gamma2 delta OC alpha d EQ Tshow.
+- unfold set_bury in EQ.
+  subst.
+  apply Tshow.
+- unfold set_bury in EQ;
+  fold @set_bury in EQ.
+  apply (IHLN _ _ _ _ _ _ EQ), cpl_tree_ex_r, Tshow.
+Qed.
+
+Lemma cpl_tree_comm_right :
+  forall {gamma delta1 delta2 : list formula} {OC : constraint} {alpha : ordinal} {d : nat},
+      (perm delta1 delta2) ->
+          showable OC gamma delta1 alpha d ->
+              showable OC gamma delta2 alpha d.
+Proof.
+intros gamma delta1 delta2 OC alpha d perm.
+pose proof (set_bury_eq_perm perm) as [LN EQ].
+apply (commutative_right_aux EQ).
+Defined.
+
+Lemma prove_dups_right_aux :
+  forall {n : nat} {gamma delta : list formula} {OC : constraint} {alpha: ordinal} {d : nat},
+      length delta = n ->
+          showable OC gamma delta alpha d ->
+              showable OC gamma (nodup form_eq_dec delta) alpha d.
+Proof.
+induction n;
+intros gamma delta OC alpha d EQ Tshow.
+- destruct delta.
+  apply Tshow.
+  inversion EQ.
+- case (no_dup_dec_cases form_eq_dec delta) as [NDD | DD].
+  + rewrite (nodup_fixed_point _ NDD).
+    apply Tshow.
+  + destruct (has_dups_split form_eq_dec DD) as [A [delta1 [delta2 [delta3 EQL]]]].
+    subst.
+    apply (cpl_tree_comm_right (perm_sym (perm_nodup form_eq_dec double_perm_head))).
+    rewrite nodup_double_cons.
+    apply IHn, cpl_tree_con_r, (cpl_tree_comm_right (double_perm_head)), Tshow.
+    rewrite app_length in EQ.
+    unfold length in *;
+    fold (@length formula) in *.
+    repeat rewrite app_length in *.
+    unfold length in EQ;
+    fold (@length formula) in EQ.
+    repeat rewrite <- plus_n_Sm in EQ.
+    lia.
+Qed.
+
+Lemma cpl_tree_nodups_right :
+  forall {gamma delta : list formula} {OC : constraint} {alpha: ordinal} {d : nat},
+      showable OC gamma delta alpha d ->
+          showable OC gamma (nodup form_eq_dec delta) alpha d.
+Proof.
+intros gamma delta OC alpha d Tshow.
+apply (prove_dups_right_aux eq_refl Tshow).
+Qed.
+
+Lemma prove_extras_right_aux :
+  forall {n : nat} {gamma delta : list formula} {OC : constraint} {alpha: ordinal} {d : nat},
+      length delta = n ->
+          showable OC gamma (nodup form_eq_dec delta) alpha d ->
+              {d' : nat & showable OC gamma delta alpha d'}.
+Proof.
+induction n;
+intros gamma delta OC alpha d EQ Tshow.
+- destruct delta.
+  refine (existT _ d Tshow).
+  inversion EQ.
+- case (no_dup_dec_cases form_eq_dec delta) as [NDD | DD].
+  + rewrite <- (nodup_fixed_point form_eq_dec NDD).
+    refine (existT _ d Tshow).
+  + destruct (has_dups_split form_eq_dec DD) as [A [delta1 [delta2 [delta3 EQL]]]].
+    subst.
+    destruct (@nodup_split_perm _ form_eq_dec (A :: A :: delta1 ++ delta2 ++ delta3)) as [pi [PERM SUB]].
+    assert (incl (flat_map vars_in pi) (OC_list OC)) as SUB'.
+    { destruct Tshow as [T [[[[[Tstr Tgam] Tdelt] Tcon] Tdeg] Tdep]].
+      refine (incl_tran (@flat_map_incl _ _ form_eq_dec nat_eq_dec _ _ _ (incl_tran SUB (incl_tran (fun B IN => perm_in form_eq_dec (perm_sym double_perm_head) _ IN) (fun B IN => proj2 (nodup_In _ _ _) IN)))) _).
+      rewrite <- Tdelt, <- Tcon.
+      apply (snd (structured_OC_semiapp _ Tstr)). }
+    apply (existT _ (length pi + d) (cpl_tree_comm_right (perm_trans _ _ _ (perm_sym PERM) (perm_sym double_perm_head)) (cpl_tree_weaken_right SUB' ((cpl_tree_comm_right (perm_nodup form_eq_dec double_perm_head)) Tshow)))).
+Qed.
+
+Lemma cpl_tree_redups_right :
+  forall {gamma delta : list formula} {OC : constraint} {alpha: ordinal} {d : nat},
+      showable OC gamma (nodup form_eq_dec delta) alpha d ->
+          {d' : nat & showable OC gamma delta alpha d'}.
+Proof.
+intros gamma delta OC alpha d Tshow.
+apply (prove_extras_right_aux eq_refl Tshow).
+Qed.
+
+Lemma cpl_tree_equiv_right :
+  forall {gamma delta1 delta2 : list formula} {OC : constraint} {alpha : ordinal} {d : nat},
+      (forall A : formula, In A delta1 <-> In A delta2) ->
+          showable OC gamma delta1 alpha d ->
+              {d' : nat & showable OC gamma delta2 alpha d'}.
+Proof.
+intros gamma delta1 delta2 OC alpha d EQUIV Tshow.
+apply (cpl_tree_redups_right ((cpl_tree_comm_right (equiv_nodup_perm form_eq_dec EQUIV)) (cpl_tree_nodups_right Tshow))).
+Qed.
+
+
+Lemma strong_ind_type :
+  forall n (P : nat -> Type), (forall n, (forall m, m < n -> P m) -> P n) -> P n.
+Proof.
+  exact (fun p P F => induction_ltof1 nat (fun m => m) P F p).
+Defined.
+
+Lemma cpl_tree_imp_l_inv_2 :
+forall {n : nat} {T : cpl_tree} {gamma delta : list formula} {phi psi : formula} {OC : constraint} {alpha : ordinal} {d : nat},
+    n = length gamma ->
+        T_shows T OC (imp phi psi :: gamma) delta alpha d ->
+            showable OC gamma (phi :: delta) alpha d.
+Proof.
+induction n as [n IND] using strong_ind_type.
+induction T;
+intros gamma' delta' phi' psi' OC' alpha' d' EQL Tshow;
+inversion Tshow as [[[[[Tstr Tgam] Tdelt] Tcon] Tdeg] Tdepth].
+
+1 : destruct Tstr as [TG_app TD_app].
+2-8 : destruct Tstr as [Tstr [[[[[TG_app TD_app] TG] TD] TOC] TDeg]].
+9 : destruct Tstr as [Tstr [[[[[[[TG_app TD_app] TG] TD] KNING] KNIND] [KIN TOC]] TDeg]].
+10 : destruct Tstr as [Tstr [[[[[[TG_app TD_app] TG] TD] TOC] TOC_rel] TDeg]].
+11 : destruct Tstr as [Tstr [[[[[[TG_app TD_app] TG] TD] [NEW [KIN TOC]]] [NING NIND]] TDeg]].
+12 : destruct Tstr as [[T1str T2str] [[[[[[[[[TG_app TD_app] T1G] T1D] T1OC] T2G] T2D] T2OC] T1Deg] T2Deg]].
+13 : destruct Tstr as [Tstr [[[[[TG_app TD_app] TG] TD] TOC] TDeg]].
+14 : destruct Tstr as [[T1str T2str] [[[[[[[[[TG_app TD_app] T1G] T1D] T1OC] T2G] T2D] T2OC] T1Deg] T2Deg]].
+
+all : unfold cpl_tree_left in Tgam;
+      subst.
+
+1 : refine (existT _ (leaf OC gamma' (phi' :: delta) alpha) _).
+    repeat split.
+    refine (fun o IN => TG_app o (in_or_app _ _ _ (or_intror IN))).
+    intros o IN.
+    apply in_app_or in IN as [IN1 | IN2].
+    refine (TG_app o (in_or_app _ _ _ (or_introl (in_or_app _ _ _ (or_introl IN1))))).
+    refine (TD_app o IN2).
+
+1 : assert (T_shows T (cpl_tree_constraint T) (imp phi' psi' :: gamma') (cpl_tree_right T) (cpl_tree_deg T) (cpl_tree_depth T)) as Tshow'.
+    { repeat split.
+      apply Tstr.
+      apply Tgam. }
+    apply cpl_tree_deg_up.
+    unfold cpl_tree_constraint at 1, cpl_tree_right at 1.
+    unfold cpl_tree_depth.
+    fold cpl_tree_depth.
+    apply (IHT _ _ _ _ _ _ _ eq_refl Tshow').
+
+1 : assert (T_shows T (cpl_tree_constraint T) (imp phi' psi' :: imp phi' psi' :: gamma') (cpl_tree_right T) (cpl_tree_deg T) (cpl_tree_depth T)) as Tshow'.
+    { repeat split.
+      apply Tstr.
+      inversion Tgam as [[EQ1 EQ2]].
+      subst.
+      apply TG. }
+    apply cpl_tree_con_r.
+    unfold cpl_tree_constraint at 1, cpl_tree_right at 1, cpl_tree_deg at 1.
+    unfold cpl_tree_depth.
+    fold cpl_tree_depth.
+    pose proof (IHT _ _ _ _ _ _ _ _ Tshow').
+
+Lemma cpl_tree_imp_l_inv_2 :
+forall {gamma delta : list formula} {phi psi : formula} {OC : constraint} {alpha : ordinal} {d : nat},
+    showable OC (imp phi psi :: gamma) delta alpha d ->
+        showable OC gamma (phi :: delta) alpha d.
+Proof.
+induction gamma;
+intros delta' phi' psi' OC' alpha' d' [T Tshow];
+inversion Tshow as [[[[[Tstr Tgam] Tdelt] Tcon] Tdeg] Tdepth].
+
+induction T.
+
+1 : destruct Tstr as [TG_app TD_app].
+2-8 : destruct Tstr as [Tstr [[[[[TG_app TD_app] TG] TD] TOC] TDeg]].
+9 : destruct Tstr as [Tstr [[[[[[[TG_app TD_app] TG] TD] KNING] KNIND] [KIN TOC]] TDeg]].
+10 : destruct Tstr as [Tstr [[[[[[TG_app TD_app] TG] TD] TOC] TOC_rel] TDeg]].
+11 : destruct Tstr as [Tstr [[[[[[TG_app TD_app] TG] TD] [NEW [KIN TOC]]] [NING NIND]] TDeg]].
+12 : destruct Tstr as [[T1str T2str] [[[[[[[[[TG_app TD_app] T1G] T1D] T1OC] T2G] T2D] T2OC] T1Deg] T2Deg]].
+13 : destruct Tstr as [Tstr [[[[[TG_app TD_app] TG] TD] TOC] TDeg]].
+14 : destruct Tstr as [[T1str T2str] [[[[[[[[[TG_app TD_app] T1G] T1D] T1OC] T2G] T2D] T2OC] T1Deg] T2Deg]].
+
+all : unfold cpl_tree_left in Tgam;
+      subst.
+
+1 : refine (existT _ (leaf OC [] (phi' :: delta) alpha) _).
+    repeat split.
+    intros o IN.
+    inversion IN.
+    intros o IN.
+    apply in_app_or in IN as [IN1 | IN2].
+    refine (TG_app o (in_or_app _ _ _ (or_introl (in_or_app _ _ _ (or_introl IN1))))).
+    refine (TD_app o IN2).
+
+1 : assert (T_shows T (cpl_tree_constraint T) (imp phi' psi' :: []) (cpl_tree_right T) (cpl_tree_deg T) (cpl_tree_depth T)) as Tshow'.
+    { repeat split.
+      apply Tstr.
+      apply Tgam. }
+    apply cpl_tree_deg_up.
+    unfold cpl_tree_constraint at 1, cpl_tree_right at 1.
+    simpl in IHT.
+    unfold cpl_tree_depth.
+    fold cpl_tree_depth.
+    apply (IHT _ _ _ _ _ _ _).
+
+
+1 : destruct Tstr as [TG_app TD_app].
+2-8 : destruct Tstr as [Tstr [[[[[TG_app TD_app] TG] TD] TOC] TDeg]].
+9 : destruct Tstr as [Tstr [[[[[[[TG_app TD_app] TG] TD] KNING] KNIND] [KIN TOC]] TDeg]].
+10 : destruct Tstr as [Tstr [[[[[[TG_app TD_app] TG] TD] TOC] TOC_rel] TDeg]].
+11 : destruct Tstr as [Tstr [[[[[[TG_app TD_app] TG] TD] [NEW [KIN TOC]]] [NING NIND]] TDeg]].
+12 : destruct Tstr as [[T1str T2str] [[[[[[[[[TG_app TD_app] T1G] T1D] T1OC] T2G] T2D] T2OC] T1Deg] T2Deg]].
+13 : destruct Tstr as [Tstr [[[[[TG_app TD_app] TG] TD] TOC] TDeg]].
+14 : destruct Tstr as [[T1str T2str] [[[[[[[[[TG_app TD_app] T1G] T1D] T1OC] T2G] T2D] T2OC] T1Deg] T2Deg]].
+
+all : unfold cpl_tree_left in TG_app, Tgam;
+    unfold cpl_tree_right in TD_app, Tdelt;
+    unfold cpl_tree_constraint in Tcon;
+    unfold cpl_tree_deg in Tdeg;
+    unfold cpl_tree_depth in Tdepth;
+    fold cpl_tree_depth in Tdepth;
+    subst.
+
+1 : refine (existT _ (leaf OC' gamma' (phi' :: delta') alpha') _).
+  repeat split.
+  refine (fun o IN => TG_app o (in_or_app _ _ _ (or_intror IN))).
+  intros o IN.
+  apply in_app_or in IN as [IN1 | IN2].
+  refine (TG_app o (in_or_app _ _ _ (or_introl (in_or_app _ _ _ (or_introl IN1))))).
+  refine (TD_app o IN2).
+
+1 : assert (T_shows T (cpl_tree_constraint T) (imp phi' psi' :: gamma') (cpl_tree_right T) (cpl_tree_deg T) (cpl_tree_depth T)) as Tshow'.
+  { repeat split.
+    apply Tstr.
+    apply Tgam. }
+  apply cpl_tree_deg_up.
+  apply (IHT _ _ _ _ _ _ _ Tshow').
+
+
+
+Qed.
+
+
+Lemma cpl_tree_imp_l_inv_2 :
+  forall {T : cpl_tree} {gamma delta : list formula} {phi psi : formula} {OC : constraint} {alpha : ordinal} {d : nat},
+      T_shows T OC (imp phi psi :: gamma) delta alpha d ->
+          showable OC gamma (phi :: delta) alpha d.
+Proof.
+induction T;
+intros gamma' delta' phi' psi' OC' alpha' d' Tshow;
+inversion Tshow as [[[[[Tstr Tgam] Tdelt] Tcon] Tdeg] Tdepth].
+
+1 : destruct Tstr as [TG_app TD_app].
+2-8 : destruct Tstr as [Tstr [[[[[TG_app TD_app] TG] TD] TOC] TDeg]].
+9 : destruct Tstr as [Tstr [[[[[[[TG_app TD_app] TG] TD] KNING] KNIND] [KIN TOC]] TDeg]].
+10 : destruct Tstr as [Tstr [[[[[[TG_app TD_app] TG] TD] TOC] TOC_rel] TDeg]].
+11 : destruct Tstr as [Tstr [[[[[[TG_app TD_app] TG] TD] [NEW [KIN TOC]]] [NING NIND]] TDeg]].
+12 : destruct Tstr as [[T1str T2str] [[[[[[[[[TG_app TD_app] T1G] T1D] T1OC] T2G] T2D] T2OC] T1Deg] T2Deg]].
+13 : destruct Tstr as [Tstr [[[[[TG_app TD_app] TG] TD] TOC] TDeg]].
+14 : destruct Tstr as [[T1str T2str] [[[[[[[[[TG_app TD_app] T1G] T1D] T1OC] T2G] T2D] T2OC] T1Deg] T2Deg]].
+
+all : unfold cpl_tree_left in TG_app, Tgam;
+      unfold cpl_tree_right in TD_app, Tdelt;
+      unfold cpl_tree_constraint in Tcon;
+      unfold cpl_tree_deg in Tdeg;
+      unfold cpl_tree_depth in Tdepth;
+      fold cpl_tree_depth in Tdepth;
+      subst.
+
+1 : refine (existT _ (leaf OC' gamma' (phi' :: delta') alpha') _).
+    repeat split.
+    refine (fun o IN => TG_app o (in_or_app _ _ _ (or_intror IN))).
+    intros o IN.
+    apply in_app_or in IN as [IN1 | IN2].
+    refine (TG_app o (in_or_app _ _ _ (or_introl (in_or_app _ _ _ (or_introl IN1))))).
+    refine (TD_app o IN2).
+
+1 : assert (T_shows T (cpl_tree_constraint T) (imp phi' psi' :: gamma') (cpl_tree_right T) (cpl_tree_deg T) (cpl_tree_depth T)) as Tshow'.
+    { repeat split.
+      apply Tstr.
+      apply Tgam. }
+    apply cpl_tree_deg_up.
+    apply (IHT _ _ _ _ _ _ _ Tshow').
+
+
+
+Qed.
+
+
+Lemma cpl_tree_imp_l_inv_2 :
+  forall {gamma delta : list formula} {phi psi : formula} {OC : constraint} {alpha : ordinal} {d : nat},
+      showable OC (imp phi psi :: gamma) delta alpha d ->
+          showable OC gamma (phi :: delta) alpha d.
+Proof.
+intros gamma delta phi psi OC alpha d Tshow.
+apply (cpl_tree_redups_right ((cpl_tree_comm_right (equiv_nodup_perm form_eq_dec EQUIV)) (cpl_tree_nodups_right Tshow))).
+Qed.
+
 (*
 Master destruct tactic.
 
 1 : destruct Tstr as [TG_app TD_app].
-2-7 : destruct Tstr as [Tstr [[[[[TG_app TD_app] TG] TD] TOC] TDeg]].
-8 : destruct Tstr as [Tstr [[[[[[[TG_app TD_app] TG] TD] KNING] KNIND] [KIN TOC]] TDeg]].
-9 : destruct Tstr as [Tstr [[[[[[TG_app TD_app] TG] TD] TOC] TOC_rel] TDeg]].
-10 : destruct Tstr as [Tstr [[[[[[TG_app TD_app] TG] TD] [NEW [KIN TOC]]] [NING NIND]] TDeg]].
-11 : destruct Tstr as [[T1str T2str] [[[[[[[[[TG_app TD_app] T1G] T1D] T1OC] T2G] T2D] T2OC] T1Deg] T2Deg]].
-12 : destruct Tstr as [Tstr [[[[[TG_app TD_app] TG] TD] TOC] TDeg]].
-13 : destruct Tstr as [[T1str T2str] [[[[[[[[[TG_app TD_app] T1G] T1D] T1OC] T2G] T2D] T2OC] T1Deg] T2Deg]].
+2-8 : destruct Tstr as [Tstr [[[[[TG_app TD_app] TG] TD] TOC] TDeg]].
+9 : destruct Tstr as [Tstr [[[[[[[TG_app TD_app] TG] TD] KNING] KNIND] [KIN TOC]] TDeg]].
+10 : destruct Tstr as [Tstr [[[[[[TG_app TD_app] TG] TD] TOC] TOC_rel] TDeg]].
+11 : destruct Tstr as [Tstr [[[[[[TG_app TD_app] TG] TD] [NEW [KIN TOC]]] [NING NIND]] TDeg]].
+12 : destruct Tstr as [[T1str T2str] [[[[[[[[[TG_app TD_app] T1G] T1D] T1OC] T2G] T2D] T2OC] T1Deg] T2Deg]].
+13 : destruct Tstr as [Tstr [[[[[TG_app TD_app] TG] TD] TOC] TDeg]].
+14 : destruct Tstr as [[T1str T2str] [[[[[[[[[TG_app TD_app] T1G] T1D] T1OC] T2G] T2D] T2OC] T1Deg] T2Deg]].
 
 *)
