theories/Logic/cpl_imp_l_inv_1.v
@@ -1,0 +1,466 @@
+From Cyclic_PA.Maths Require Import naturals.
+From Cyclic_PA.Maths Require Import ordinals.
+From Cyclic_PA.Maths Require Import lists.
+From Cyclic_PA.Logic Require Import definitions.
+From Cyclic_PA.Logic Require Import constraints.
+From Cyclic_PA.Logic Require Import fol.
+From Cyclic_PA.Logic Require Import substitute.
+From Cyclic_PA.Logic Require Import proof_trees.
+From Cyclic_PA.Logic Require Import cpl_trees.
+Require Import Lia.
+Require Import List.
+Import ListNotations.
+Require Import Coq.Logic.ProofIrrelevance.
+Require Import Coq.Logic.Eqdep_dec.
+Require Import Arith.
+
+Definition imp_left_inv_1_formula (phi A B : formula) (b : bool) : formula := formula_sub phi (imp A B) B b.
+
+Definition imp_left_inv_1_batch (gamma : list formula) (A B : formula) (S : subst_ind) : list formula := batch_sub gamma (imp A B) B S.
+
+Fixpoint cpl_tree_imp_l_inv_1_fit
+  (T : cpl_tree) (A B : formula) (S : subst_ind) : cpl_tree :=
+let REC := (fun PT SI => (cpl_tree_imp_l_inv_1_fit PT A B SI)) in
+match T, S with
+| leaf OC gamma delta l, _ => leaf OC (imp_left_inv_1_batch gamma A B S) delta l
+
+| @deg_up OC gamma delta alpha beta T', _ => @deg_up OC (cpl_tree_left (REC T' S)) delta alpha beta (REC T' S)
+
+| @con_l OC gamma delta phi alpha T', s :: S' => @con_l OC (imp_left_inv_1_batch gamma A B S') delta (imp_left_inv_1_formula phi A B s) alpha (REC T' (s :: s :: S'))
+
+| @con_r OC gamma delta phi alpha T', _ => @con_r OC (cpl_tree_left (REC T' S)) delta phi alpha (REC T' S)
+
+| @ex_l OC gamma delta n alpha T', _ => @ex_l OC (cpl_tree_left (REC T' (unbury S n))) delta n alpha (REC T'(unbury S n))
+
+| @ex_r OC gamma delta n alpha T', _ => @ex_r OC (cpl_tree_left (REC T' S)) delta n alpha (REC T' S)
+
+| @wkn_l OC gamma delta phi alpha T', s :: S' => @wkn_l OC (imp_left_inv_1_batch gamma A B S') delta (imp_left_inv_1_formula phi A B s) alpha (REC T' S')
+
+| @wkn_r OC gamma delta phi alpha T', _ => @wkn_r OC (cpl_tree_left (REC T' S)) delta phi alpha (REC T' S)
+
+| @rst OC gamma delta eta alpha T', _ => @rst OC (cpl_tree_left (REC T' S)) delta eta alpha (REC T' S)
+
+| @bnd_l OC gamma delta phi eta iota alpha T', s :: S' => @bnd_l OC (imp_left_inv_1_batch gamma A B S') delta phi eta iota alpha (REC T' (false :: S'))
+
+| @bnd_r OC gamma delta phi eta iota alpha T', _ => @bnd_r OC (cpl_tree_left (REC T' S)) delta phi eta iota alpha (REC T' S)
+
+| @imp_l OC gamma delta phi psi alpha1 alpha2 T1 T2, s :: S' => match (form_eqb phi A), (form_eqb psi B), s with
+    | true, true, true => @deg_up OC (cpl_tree_left (REC T1 (false :: S'))) delta alpha1 alpha2 (REC T1 (false :: S'))
+    | _, _ , _ => @imp_l OC (imp_left_inv_1_batch gamma A B S') delta phi psi alpha1 alpha2 (REC T1 (false :: S')) (REC T2 S')
+    end
+
+| @imp_r OC gamma delta phi psi alpha T', _ => @imp_r OC (imp_left_inv_1_batch gamma A B S) delta phi psi alpha (REC T' (false :: S))
+
+| @cut OC gamma delta phi alpha1 alpha2 T1 T2, _ => @cut OC (imp_left_inv_1_batch gamma A B S) delta phi alpha1 alpha2 (REC T1 S) (REC T2 (false :: S))
+
+| _ , _ => T
+end.
+
+Definition cpl_tree_imp_l_inv_1 (T : cpl_tree) (A B : formula) (S : subst_ind) : cpl_tree :=
+match nat_eqb (length (cpl_tree_left T)) (length S) with
+| true => cpl_tree_imp_l_inv_1_fit T A B S
+| false => T
+end.
+
+
+Lemma cpl_tree_imp_l_inv_1_fit_true :
+    forall {T : cpl_tree} {A B : formula},
+        forall {S : subst_ind},
+            nat_eqb (length (cpl_tree_left T)) (length S) = true ->
+                (cpl_tree_imp_l_inv_1_fit T A B S) = (cpl_tree_imp_l_inv_1 T A B S).
+Proof. intros T A B S EQ. unfold cpl_tree_imp_l_inv_1. rewrite EQ. reflexivity. Qed.
+
+Lemma cpl_tree_imp_l_inv_1_left :
+    forall (T : cpl_tree) (A B : formula),
+        structured T ->
+            forall (S : subst_ind),
+                cpl_tree_left (cpl_tree_imp_l_inv_1 T A B S) =
+                    (imp_left_inv_1_batch (cpl_tree_left T) A B S).
+Proof.
+intros T A B.
+induction T;
+try intros Tstr S;
+unfold cpl_tree_imp_l_inv_1;
+unfold imp_left_inv_1_batch, batch_sub;
+case nat_eqb eqn:EQ;
+try reflexivity;
+unfold cpl_tree_imp_l_inv_1_fit;
+fold cpl_tree_imp_l_inv_1_fit;
+unfold cpl_tree_left in EQ;
+fold cpl_tree_left in EQ.
+
+1 : destruct Tstr as [TG_app TD_app].
+2-8 : destruct Tstr as [Tstr [[[[[TG_app TD_app] TG] TD] TOC] TDeg]].
+9 : destruct Tstr as [Tstr [[[[[[[TG_app TD_app] TG] TD] KNING] KNIND] [KIN TOC]] TDeg]].
+10 : destruct Tstr as [Tstr [[[[[[TG_app TD_app] TG] TD] TOC] TOC_rel] TDeg]].
+11 : destruct Tstr as [Tstr [[[[[[TG_app TD_app] TG] TD] [NEW [KIN TOC]]] [NING NIND]] TDeg]].
+12 : destruct Tstr as [[T1str T2str] [[[[[[[[[TG_app TD_app] T1G] T1D] T1OC] T2G] T2D] T2OC] T1Deg] T2Deg]].
+13 : destruct Tstr as [Tstr [[[[[TG_app TD_app] TG] TD] TOC] TDeg]].
+14 : destruct Tstr as [[T1str T2str] [[[[[[[[[TG_app TD_app] T1G] T1D] T1OC] T2G] T2D] T2OC] T1Deg] T2Deg]].
+
+all : subst;
+      unfold cpl_tree_left;
+      unfold batch_sub_fit;
+      fold @batch_sub_fit.
+
+all : try rewrite (batch_sub_fit_true EQ);
+      try rewrite (cpl_tree_imp_l_inv_1_fit_true EQ);
+      unfold imp_left_inv_1_batch;
+      try apply (IHT Tstr);
+      try reflexivity.
+
+2 : { fold (cpl_tree_left (cpl_tree_imp_l_inv_1_fit T A B (unbury S n))).
+      rewrite cpl_tree_imp_l_inv_1_fit_true, <- batch_bury_comm, (IHT Tstr).
+      reflexivity.
+      rewrite bury_length, <- (@bury_unbury _ S n), bury_length in EQ.
+      apply EQ. }
+
+all : destruct S as [ | b S];
+      inversion EQ as [EQ'];
+      unfold length in *;
+      fold (@length bool) (@length formula) in *.
+
+4 : case (form_eqb phi A) eqn:EQF1;
+    try apply form_eqb_eq in EQF1.
+4 : case (form_eqb psi B) eqn:EQF2;
+    try apply form_eqb_eq in EQF2.
+4 : destruct b.
+
+all : subst;
+      unfold cpl_tree_left;
+      try fold (cpl_tree_left T);
+      try fold (cpl_tree_left T2);
+      unfold batch_sub, batch_sub_fit;
+      fold batch_sub_fit;
+      try rewrite batch_sub_fit_true;
+      try rewrite TG;
+      try rewrite EQ';
+      try rewrite EQ;
+      try apply EQ;
+      try reflexivity.
+
+1 : fold (cpl_tree_left (cpl_tree_imp_l_inv_1_fit T1 A B (false :: S))).
+    rewrite cpl_tree_imp_l_inv_1_fit_true, (IHT1 T1str).
+    unfold formula_sub.
+    rewrite form_eqb_refl, T1G.
+    unfold imp_left_inv_1_batch.
+    apply batch_sub_false_head.
+    rewrite T1G.
+    apply EQ'.
+
+all : unfold formula_sub, form_eqb, imp_left_inv_1_batch, batch_sub, batch_sub_fit at 1;
+      fold batch_sub_fit form_eqb;
+      try rewrite EQ';
+      try rewrite !form_eqb_refl;
+      try rewrite EQF1;
+      try rewrite EQF2;
+      try rewrite !andb_false_r;
+      try rewrite !andb_false_l;
+      try reflexivity.
+Qed.
+
+Lemma cpl_tree_imp_l_inv_1_right :
+    forall (T : cpl_tree) (A B : formula),
+        structured T ->
+            forall (S : subst_ind),
+                cpl_tree_right (cpl_tree_imp_l_inv_1 T A B S) =
+                   (cpl_tree_right T).
+Proof.
+intros T A B.
+induction T;
+try intros Tstr S;
+unfold cpl_tree_imp_l_inv_1;
+unfold imp_left_inv_1_batch, batch_sub.
+
+1 : destruct Tstr as [TG_app TD_app].
+2-8 : destruct Tstr as [Tstr [[[[[TG_app TD_app] TG] TD] TOC] TDeg]].
+9 : destruct Tstr as [Tstr [[[[[[[TG_app TD_app] TG] TD] KNING] KNIND] [KIN TOC]] TDeg]].
+10 : destruct Tstr as [Tstr [[[[[[TG_app TD_app] TG] TD] TOC] TOC_rel] TDeg]].
+11 : destruct Tstr as [Tstr [[[[[[TG_app TD_app] TG] TD] [NEW [KIN TOC]]] [NING NIND]] TDeg]].
+12 : destruct Tstr as [[T1str T2str] [[[[[[[[[TG_app TD_app] T1G] T1D] T1OC] T2G] T2D] T2OC] T1Deg] T2Deg]].
+13 : destruct Tstr as [Tstr [[[[[TG_app TD_app] TG] TD] TOC] TDeg]].
+14 : destruct Tstr as [[T1str T2str] [[[[[[[[[TG_app TD_app] T1G] T1D] T1OC] T2G] T2D] T2OC] T1Deg] T2Deg]].
+
+all : subst; 
+      case nat_eqb eqn:EQ;
+      try reflexivity;
+      unfold cpl_tree_imp_l_inv_1_fit;
+      fold cpl_tree_imp_l_inv_1_fit;
+      unfold cpl_tree_left in EQ;
+      fold cpl_tree_left in EQ.
+
+all : destruct S as [ | b S];
+      inversion EQ;
+      try case (form_eqb phi A) eqn:EQF1;
+      try case (form_eqb psi B) eqn:EQF2;
+      destruct b;
+      try reflexivity.
+Qed.
+
+Lemma cpl_tree_imp_l_inv_1_constraint :
+    forall (T : cpl_tree) (A B : formula),
+        structured T ->
+            forall (S : subst_ind),
+                cpl_tree_constraint (cpl_tree_imp_l_inv_1 T A B S) =
+                   (cpl_tree_constraint T).
+Proof.
+intros T A B.
+induction T;
+try intros Tstr S;
+unfold cpl_tree_imp_l_inv_1;
+unfold imp_left_inv_1_batch, batch_sub.
+
+1 : destruct Tstr as [TG_app TD_app].
+2-8 : destruct Tstr as [Tstr [[[[[TG_app TD_app] TG] TD] TOC] TDeg]].
+9 : destruct Tstr as [Tstr [[[[[[[TG_app TD_app] TG] TD] KNING] KNIND] [KIN TOC]] TDeg]].
+10 : destruct Tstr as [Tstr [[[[[[TG_app TD_app] TG] TD] TOC] TOC_rel] TDeg]].
+11 : destruct Tstr as [Tstr [[[[[[TG_app TD_app] TG] TD] [NEW [KIN TOC]]] [NING NIND]] TDeg]].
+12 : destruct Tstr as [[T1str T2str] [[[[[[[[[TG_app TD_app] T1G] T1D] T1OC] T2G] T2D] T2OC] T1Deg] T2Deg]].
+13 : destruct Tstr as [Tstr [[[[[TG_app TD_app] TG] TD] TOC] TDeg]].
+14 : destruct Tstr as [[T1str T2str] [[[[[[[[[TG_app TD_app] T1G] T1D] T1OC] T2G] T2D] T2OC] T1Deg] T2Deg]].
+
+all : subst; 
+      case nat_eqb eqn:EQ;
+      try reflexivity;
+      unfold cpl_tree_imp_l_inv_1_fit;
+      fold cpl_tree_imp_l_inv_1_fit;
+      unfold cpl_tree_left in EQ;
+      fold cpl_tree_left in EQ.
+
+all : destruct S as [ | b S];
+      inversion EQ;
+      try case (form_eqb phi A) eqn:EQF1;
+      try case (form_eqb psi B) eqn:EQF2;
+      destruct b;
+      try reflexivity.
+Qed.
+
+Lemma cpl_tree_imp_l_inv_1_deg :
+    forall (T : cpl_tree) (A B : formula),
+        structured T ->
+            forall (S : subst_ind),
+                cpl_tree_deg (cpl_tree_imp_l_inv_1 T A B S) =
+                   (cpl_tree_deg T).
+Proof.
+intros T A B.
+induction T;
+try intros Tstr S;
+unfold cpl_tree_imp_l_inv_1;
+unfold imp_left_inv_1_batch, batch_sub.
+
+1 : destruct Tstr as [TG_app TD_app].
+2-8 : destruct Tstr as [Tstr [[[[[TG_app TD_app] TG] TD] TOC] TDeg]].
+9 : destruct Tstr as [Tstr [[[[[[[TG_app TD_app] TG] TD] KNING] KNIND] [KIN TOC]] TDeg]].
+10 : destruct Tstr as [Tstr [[[[[[TG_app TD_app] TG] TD] TOC] TOC_rel] TDeg]].
+11 : destruct Tstr as [Tstr [[[[[[TG_app TD_app] TG] TD] [NEW [KIN TOC]]] [NING NIND]] TDeg]].
+12 : destruct Tstr as [[T1str T2str] [[[[[[[[[TG_app TD_app] T1G] T1D] T1OC] T2G] T2D] T2OC] T1Deg] T2Deg]].
+13 : destruct Tstr as [Tstr [[[[[TG_app TD_app] TG] TD] TOC] TDeg]].
+14 : destruct Tstr as [[T1str T2str] [[[[[[[[[TG_app TD_app] T1G] T1D] T1OC] T2G] T2D] T2OC] T1Deg] T2Deg]].
+
+all : subst; 
+      case nat_eqb eqn:EQ;
+      try reflexivity;
+      unfold cpl_tree_imp_l_inv_1_fit;
+      fold cpl_tree_imp_l_inv_1_fit;
+      unfold cpl_tree_left in EQ;
+      fold cpl_tree_left in EQ.
+
+all : destruct S as [ | b S];
+      inversion EQ;
+      try case (form_eqb phi A) eqn:EQF1;
+      try case (form_eqb psi B) eqn:EQF2;
+      destruct b;
+      try reflexivity.
+Qed.
+
+
+Lemma imp_l_formula_inv_1_vars_in :
+    forall (phi : formula) (A B : formula) (b : bool) (OC : constraint),
+        incl (vars_in phi) (OC_list OC) ->
+            incl (vars_in (imp_left_inv_1_formula phi A B b)) (OC_list OC).
+Proof.
+intros phi A B b OC SUB o IN.
+unfold imp_left_inv_1_formula, formula_sub in IN.
+apply SUB.
+case form_eqb eqn:EQF.
+destruct b.
+apply form_eqb_eq in EQF.
+subst.
+apply in_or_app,or_intror.
+all : apply IN.
+Qed.
+
+Lemma cpl_tree_imp_l_inv_1_vars_in :
+    forall {gamma : list formula} {A B : formula} (S : subst_ind) {OC : constraint},
+        incl (flat_map vars_in gamma) (OC_list OC) ->
+            incl (flat_map vars_in (imp_left_inv_1_batch gamma A B S)) (OC_list OC).
+Proof.
+induction gamma;
+intros A B S OC SUB;
+unfold imp_left_inv_1_batch, batch_sub, batch_sub_fit;
+fold batch_sub_fit;
+destruct S;
+unfold length, nat_eqb;
+fold (@length formula) (@length bool) nat_eqb.
+4 : case nat_eqb eqn:EQN.
+1,2,3,5 : apply SUB.
+unfold flat_map;
+fold (flat_map vars_in).
+rewrite (batch_sub_fit_true EQN).
+fold (imp_left_inv_1_batch gamma A B S).
+apply incl_app_inv in SUB as [SUB1 SUB2].
+apply (incl_app (imp_l_formula_inv_1_vars_in _ _ _ _ _ SUB1) (IHgamma _ _ _ _ SUB2)).
+Qed.
+
+
+Lemma imp_l_formula_inv_1_vars_used_sub :
+    forall {phi : formula} {A B : formula} {b : bool},
+        incl (vars_used (imp_left_inv_1_formula phi A B b)) (vars_used phi).
+Proof.
+intros phi A B b o IN.
+unfold imp_left_inv_1_formula, formula_sub in IN.
+case form_eqb eqn:EQF.
+destruct b.
+apply form_eqb_eq in EQF.
+subst.
+apply in_or_app,or_intror.
+all : apply IN.
+Qed.
+
+Lemma imp_l_formula_inv_1_vars_used_sub_batch :
+    forall {gamma : list formula} {A B : formula} {S : subst_ind},
+        incl (flat_map vars_used (imp_left_inv_1_batch gamma A B S)) (flat_map vars_used gamma).
+Proof.
+induction gamma;
+intros A B S o IN;
+destruct S;
+try contradiction IN;
+unfold imp_left_inv_1_batch, batch_sub, batch_sub_fit, length, nat_eqb in IN.
+apply IN.
+fold (@length formula) (@length bool) nat_eqb batch_sub_fit in IN.
+case nat_eqb eqn:EQL.
+2 : apply IN.
+rewrite (batch_sub_fit_true EQL) in IN.
+apply in_app_or in IN as [IN1 | IN2].
+apply in_or_app, or_introl, (imp_l_formula_inv_1_vars_used_sub _ IN1).
+apply in_or_app, or_intror, (IHgamma _ _ _ _ IN2).
+Qed.
+
+Lemma cpl_tree_imp_l_inv_1_struct_aux :
+    forall (T : cpl_tree) (A B : formula),
+        structured T ->
+            forall (S : subst_ind),
+                structured (cpl_tree_imp_l_inv_1 T A B S).
+Proof.
+intros T A B.
+induction T;
+try intros Tstr S;
+unfold cpl_tree_imp_l_inv_1;
+unfold imp_left_inv_1_batch, batch_sub.
+
+1 : destruct Tstr as [TG_app TD_app].
+2-8 : destruct Tstr as [Tstr [[[[[TG_app TD_app] TG] TD] TOC] TDeg]].
+9 : destruct Tstr as [Tstr [[[[[[[TG_app TD_app] TG] TD] KNING] KNIND] [KIN TOC]] TDeg]].
+10 : destruct Tstr as [Tstr [[[[[[TG_app TD_app] TG] TD] TOC] TOC_rel] TDeg]].
+11 : destruct Tstr as [Tstr [[[[[[TG_app TD_app] TG] TD] [NEW [KIN TOC]]] [NING NIND]] TDeg]].
+12 : destruct Tstr as [[T1str T2str] [[[[[[[[[TG_app TD_app] T1G] T1D] T1OC] T2G] T2D] T2OC] T1Deg] T2Deg]].
+13 : destruct Tstr as [Tstr [[[[[TG_app TD_app] TG] TD] TOC] TDeg]].
+14 : destruct Tstr as [[T1str T2str] [[[[[[[[[TG_app TD_app] T1G] T1D] T1OC] T2G] T2D] T2OC] T1Deg] T2Deg]].
+
+all : subst; 
+      case nat_eqb eqn:EQ;
+      unfold cpl_tree_imp_l_inv_1_fit;
+      fold cpl_tree_imp_l_inv_1_fit;
+      unfold cpl_tree_left in EQ;
+      fold cpl_tree_left in EQ;
+      try fold (cpl_tree_left T) in EQ;
+      try fold (cpl_tree_left T1) in EQ;
+      try fold (cpl_tree_left T2) in EQ.
+
+5,13,19,23 : destruct S.
+
+12 : case (form_eqb phi A) eqn:FEQ1.
+12 : case (form_eqb psi B) eqn:FEQ2.
+12 : destruct b.
+
+2,4,5,7,9,11,16,18,20,22,23,25,27,28,30,31,33,35 : repeat split; try assumption; try apply (existT _ NEW (existT _ KIN TOC)).
+
+14 :  { rewrite cpl_tree_imp_l_inv_1_fit_true.
+        repeat split;
+        try assumption.
+        - apply (IHT Tstr).
+        - unfold cpl_tree_left at 1.
+          rewrite cpl_tree_imp_l_inv_1_left.
+          apply (cpl_tree_imp_l_inv_1_vars_in S TG_app).
+          apply Tstr.
+        - apply cpl_tree_imp_l_inv_1_right, Tstr.
+        - rewrite cpl_tree_imp_l_inv_1_left.
+          intros FAL.
+          apply KNING.
+          apply (imp_l_formula_inv_1_vars_used_sub_batch _ FAL).
+          apply Tstr.
+        - rewrite <- TOC.
+          apply cpl_tree_imp_l_inv_1_constraint, Tstr.
+        - apply cpl_tree_imp_l_inv_1_deg, Tstr.
+        - apply EQ. }
+
+all : try rewrite !cpl_tree_imp_l_inv_1_fit_true;
+      try rewrite TG;
+      try rewrite T1G;
+      try rewrite T2G;
+      try rewrite bury_length, <- (@bury_unbury _ S n), bury_length in EQ;
+      try apply EQ;
+      repeat split;
+      try apply (IHT Tstr);
+      try apply (IHT1 T1str);
+      try apply (IHT2 T2str);
+      try apply (cpl_tree_imp_l_inv_1_vars_in _ TG_app);
+      try apply (cpl_tree_imp_l_inv_1_vars_in _ TD_app);
+      try rewrite cpl_tree_imp_l_inv_1_left;
+      try rewrite cpl_tree_imp_l_inv_1_right;
+      try rewrite cpl_tree_imp_l_inv_1_constraint;
+      try rewrite cpl_tree_imp_l_inv_1_deg;
+      try refine (existT _ NEW (existT _ KIN TOC));
+      try apply Tstr;
+      try apply T1str;
+      try apply T2str;
+      try rewrite TG;
+      try rewrite T1G;
+      try rewrite T2G;
+      try rewrite TD;
+      try rewrite T1D;
+      try rewrite T2D;
+      try rewrite T1OC;
+      try rewrite T2OC;
+      try apply EQ;
+      try reflexivity;
+      unfold imp_left_inv_1_batch, batch_sub, batch_sub_fit;
+      fold batch_sub_fit;
+      unfold length, nat_eqb in *;
+      fold (@length formula) (@length bool) nat_eqb in *;
+      try rewrite EQ;
+      try rewrite formula_sub_false;
+      try reflexivity;
+      try apply TD_app;
+      try assumption.
+
+all : unfold cpl_tree_left in *;
+      unfold imp_left_inv_1_formula;
+      try fold (cpl_tree_left T) in *;
+      try fold (cpl_tree_left T2) in *;
+      try rewrite batch_sub_fold_head;
+      try rewrite batch_sub_fit_true;
+      try apply EQ;
+      try rewrite batch_bury_comm;
+      try apply (cpl_tree_imp_l_inv_1_vars_in S TG_app);
+      try apply (cpl_tree_imp_l_inv_1_vars_in (b :: S) TG_app);
+      unfold flat_map in *;
+      fold (flat_map vars_in) in *;
+      fold (flat_map vars_used) in *;
+      try apply (incl_app (proj1 (incl_app_inv _ _ TG_app)) (cpl_tree_imp_l_inv_1_vars_in _ (proj2 (incl_app_inv _ _ TG_app))));
+      try apply (incl_app (proj2 (incl_app_inv _ _ (proj1 (incl_app_inv _ _ TG_app)))) (cpl_tree_imp_l_inv_1_vars_in _ (proj2 (incl_app_inv _ _ TG_app)))).
+
+1 : intros FAL.
+    apply NING.
+    apply (imp_l_formula_inv_1_vars_used_sub_batch _ FAL).
+Qed.
